\section{oops}

\begin{align}
y(x) \approx \sum_{m=0}^M \bar{y}_m \cos\mu_m x
\end{align}

Assim:
\begin{align}
& \int_0^a Y(x)dx = a \bar{y}_0 \\ \nonumber \\
& \int_0^a Y(x)\cos\mu_m dx = \frac{a}{2}\bar{y}_m
\end{align}

\begin{align}
\Re(F_{1,j})
& =
-\frac{q}{k_1}\bar{\psi}_{j,0} + \frac{\mathbb{A}_{j,0} - \bar{\psi}_{j,0}}{b} \bar{y}_0 + \sum_{m=1}^M \mu_m \left(\frac{\mathbb{A}_{j,m}}{\sinh\mu_m b} - \frac{\bar{\psi}_{j, m}}{\tanh\mu_m b}\right)\bar{y}_m
\end{align}

E se
\begin{align}
y(x) \approx \bar{y}_0 + \sum_{m=1}^M \bar{y}_m \sin\mu_m x
\end{align}

Ent√£o
\begin{align}
& \int_0^a Y(x)dx = a \bar{y}_0 + \frac{a}{\pi}\sum_{m=1}^M \bar{y}_m \frac{1 - (-1)^m}{m} \\ \nonumber \\
& \int_0^a Y(x)\cos\mu_n dx =\frac{a}{\pi}\sum_{m=1,m\ne n}^M \bar{y}_m \frac{m[1 - (-1)^{m+n}]}{m^2 - n^2}
\end{align}